$$
P\left(\frac{X_{1}+X_{2}+\cdots+X_{n}-n \mu}{\sigma \sqrt{n}} \leq x\right)\to \frac{1}{\sqrt{2 \pi}} \int_{-\infty}^{x} e^{-t^{2} / 2} d t
$$

$$
F=G \frac{m_{1} m_{2}}{r^{2}}
$$

$$
\frac{\partial^{2} y}{\partial t^{2}}=c^{2} \frac{\partial^{2} y}{\partial x^{2}}
$$

$$
V-E+F=2
$$

$$
\Delta_{\psi}(P) \Delta_{\psi}(X) \geq \hbar
$$

$$
H(S) \leq m(S) \leq H(S)+1
$$

$$
P \stackrel{?}{=} N P
$$

$$
i \hbar \frac{\partial \psi}{\partial t}=\frac{-\hbar^{2}}{2 m} \nabla^{2} \psi+V \psi
$$

$$
\frac{1}{\pi}=\frac{\sqrt{8}}{99^{2}} \sum_{n=0}^{\infty} \frac{(4 n) !}{(n !)^{4}} \frac{(1103+26390 n)}{396^{4 n}}
$$

$$
l^{\prime}=\frac{l}{\sqrt{1-\frac{v^{2}}{c^{2}} }}
$$

$$
\frac{d N}{d t}=r N\left(1-\frac{N}{K}\right)
$$

$$
P(A)=(k/N)^n
p(B|A)=1-\sum_{i=1}^{k-1}\binom{k}{i}(1-i/k)^n(-1)^{i+1}
P\{D=k\}=\binom{N}{k}P(AB)
$$


$$
\left\{ \begin{array}{l}  U = \frac { Q } { C } = \frac { n q } { C }  \\ { a = g - \frac { E q } { m } = g - \frac { U q } { d m } = g - \frac { n q ^ { 2 } } { d m C } } \\ { \frac { d } { 2 } = \frac { 1 } { 2 } a t ^ { 2 } = \frac { 1 } { 2 } ( g - \frac { n q ^ { 2 } } { d m C } ) \cdot ( \frac { L } { v _ { 0 } } ) ^ { 2 } } \end{array} \right .\Rightarrow n = ( g - \frac { d v _ { 0 } ^ { 2 } } { L ^ { 2 } } ) \cdot \frac { d m C } { q ^ { 2 } }
$$

$$
\oint IR=0
$$

$$
\left \{\begin{array}{l}x=x_0+t\cos\theta,\\y=y_0+t\sin\theta \end{array}\right .(\theta\in [0,\pi])
$$

$$
\rho =\frac{ep}{1-e\cos\theta}
$$

$$
\frac {x^2} {a^2}\pm \frac {y^2} {b^2}=1
$$

$$
\left\{ \begin{array}{l}m\frac{v^2}{r}=Bqv\\T=\frac {2\pi r} v \end{array}\right .\Rightarrow T=\frac{2\pi m} {Bq}\Rightarrow t=\frac{\theta m} {Bq}
$$

$$
\sum_{i = 1}^{k} i ^ {2} = \frac{k {(k + 1)} {(2 k + 1)}}{6}\\
$$

$$
\begin{array} {}\sum_\limits{i = 1}^{k+1}i^{2}&= \sum_\limits{i = 1}^{k} i ^ {2}+(k+1)^2\\&= \frac{k {(k + 1)} {(2 k + 1)+6(k+1)^2}}{6}\\&=\frac{(k + 1)(2k^2+7k+6)}{6}\\&=\frac{(k + 1)[(k+1)+1][2(k+1)+1]}{6}\end{array}
$$

$$
t=(1+x)^n-1\rightarrow0\\
\begin{array} {aligned}\lim_\limits{x \to 0} \frac{(1+x)^n-1}{x}(n\in R)&=\lim_\limits{x \to 0}[\frac{(1+x)^n-1}{\ln(1+x)^n}\cdot\frac{n\ln(1+x)}{x}]\\&=\lim_\limits{x \to 0} \frac{t}{\ln(1+t)}\cdot\lim_\limits{x \to 0}\frac{n\ln(1+x)}{x}\\&=\frac 1 e\cdot e\cdot n\\&=n\end{array}\\
(1+x)^\alpha\thicksim 1+\alpha x(x\rightarrow0)
$$

$$
(1+x)^n> 1+n x\;(n>1,n\in N^*)\\
( 1 + x ) ^ { k } > 1 + k x\\
 \begin{array} {aligned} ( 1 + x ) ^ { k + 1 } &= ( 1 + x ) ( 1 + x ) ^ { k } \\&>{ ( 1 + x ) ( 1 + k x ) }\\ &={ 1 + x + k x + k x ^ { 2 } }\\ &> {1 + ( k + 1 ) x }\end{array}
$$

$$
\int^{t}_{0}\mathrm{d}t =-\int_{v_0}^{v}\frac{mR}{B^2L^2v}\mathrm{d}v
$$

$$
\int \textrm{efforts}+\texttt{immaturity}+\textrm{d}\textbf{lucky}=Success
$$

$$
\frac{d}{dx}(f(x)+g(x))=\frac {df}{dx}+\frac{dg}{dx}
$$

$$
\int_{a}^{b}f(x)dx=F(b)-F(a)
$$

$$
-2^{w-1}\le x<2^{w-1}-1\qquad \textrm{and}\qquad-2^{w-1}\le y<2^{w-1}-1\qquad\\
x+y=\left\{\begin{array}{l}x+y-2^w,\quad x+y\ge 2^{w-1}\\x+y,\quad 2^{w-1}\le x+y<2^{w-1}\\x+y-2^w,\quad x+y<-2^{w-1}\end{array}\right.
$$

$$
\textrm{binary  to  unsigned}\\
B2U_w(\overrightarrow{x})=x_{w-1}\cdot 2^{w-1}+x_{w-2}\cdot 2^{w-2}+\cdot\cdot\cdot+x_0\cdot2^0=\sum_{i=0}^{w-1}x_i\cdot 2^i
$$

$$
\textrm{binary  to  two's complement representation}\\
B2U_w(\overrightarrow{x})=x_{w-1}\cdot -2^{w-1}+x_{w-2}\cdot 2^{w-2}+\cdot\cdot\cdot+x_0\cdot2^0=x_{w-1}\cdot -2^{w-1}+\sum_{i=0}^{w-2}x_i\cdot 2^i
$$

$$
x\cdot2^k=x<<k
$$

$$
x=d_md_{m-1}…d_1d_0.d_{-1}…d_{-(n-1)}d_{-n}\\
x=\sum_{i=-n}^{m}d_i\cdot10^i
$$

$$
float=>V=(-1)^s\times M\times2^E\\
E=e-bias(bias=2^{8-1}-1=127)
\\e\in[1,255]\\E\in[-126,127]\\M=1+f=1.f_{22}f_{21…}f_1
$$

$$
\bar{F} =\frac{m_0}{l_1}\sum_{i=1}^{N}v_{ix}^2
$$

$$
p=n_0kTe^{-\frac{m_0gh}{kT}}
$$

$$
\rm Youth\;passes,but\;with\;luck\;immaturity\;can\;last\;a\;lifetime.
$$



